Actualizo BDA+VFS

Optativas/VFS/practicas/Clase3.GADT.fst
@@ -20,13 +20,14 @@ let lift (ty : l_ty) : Type =
 
 val eval (#ty:l_ty) (e : expr ty) : Tot (lift ty)
 
-let rec eval (#ty:l_ty) (e : expr ty) : Tot (lift ty) =
+let rec eval (#ty:l_ty) (e : expr ty) : Tot (lift ty) (decreases e) =
   match e with
-    | EInt i      -> i
-    | EBool b     -> b
-    | EAdd e1 e2  -> (eval e1) + (eval e2)
-    | EEq e1 e2   -> true // (eval e1) = (eval e2) 
-    | EIf c e1 e2 -> 
-      if true // eval c
-      then eval e1
-      else eval e2
+  | EInt i    -> i
+  | EBool b   -> b
+  | EAdd l r  -> eval l + eval r
+  | EEq l r   -> eval l = eval r
+  | EIf c l r -> 
+    if eval c
+    then eval l
+    else eval r
+
